Escrevendo + mudanças Coq

DFA.v
@@ -5,30 +5,30 @@ Set Implicit Arguments.
 (*Unset Strict Implicit.
 Unset Printing Implicit Defensive.*)
 
-Inductive state {Q : Type} : Type :=
-  | sink_state
-  | proper_state (q : Q).
+Inductive state {Q : Type} :=
+  sink_state | proper_state (q : Q).
 
 Record dfa (Q E : Type) := {
-  delta: Q -> E -> @state Q;
+  transition: Q -> E -> @state Q;
   initial_state: Q;
-  is_final: Q -> bool
+  is_marked: Q -> bool
 }.
 
 (* Extended transition function: *)
 
-Fixpoint extended_delta {Q E : Type} (g : dfa Q E) q w : state :=
+Fixpoint extended_transition {Q E : Type} (g : dfa Q E) q w : state :=
   match q with
-  | sink_state => sink_state
-  | proper_state q' => match w with
-                | [] => proper_state q'
-                | e::w' => extended_delta g ((delta g) q' e) w'
-                end
+    sink_state => sink_state |
+    proper_state q' =>  match w with
+                          [] => proper_state q' |
+                          e::w' =>
+                            extended_transition g ((transition g) q' e) w'
+                        end
   end.
 
-Lemma extended_delta_sink_state:
+Lemma transition_over_sink_state:
   forall (Q E : Type) (g : dfa Q E) w,
-    extended_delta g sink_state w = sink_state.
+    extended_transition g sink_state w = sink_state.
 Proof.
   intros Q E g w.
   destruct w.
@@ -36,23 +36,23 @@ Proof.
   reflexivity.
 Qed.
 
-Theorem dist_extended_delta:
+Theorem dist_extended_transition:
   forall (Q E : Type) (g : dfa Q E) w w' q,
-    extended_delta g q (w ++ w') =
-    extended_delta g (extended_delta g q w) w'.
+    extended_transition g q (w ++ w') =
+    extended_transition g (extended_transition g q w) w'.
 Proof.
   intros Q E g w.
   induction w as [|e w IHw].
   - intros w' q. simpl. destruct q. reflexivity. reflexivity.
   - intros w' q. simpl. destruct q.
-    + symmetry. apply extended_delta_sink_state.
+    + symmetry. apply transition_over_sink_state.
     + rewrite IHw. reflexivity.
 Qed.
 
 (* Generated language: *)
 
 Definition in_language {Q E : Type} (g : dfa Q E) w : Prop :=
-  ~ extended_delta g (proper_state (initial_state g)) w = sink_state.
+  ~ extended_transition g (proper_state (initial_state g)) w = sink_state.
 
 Notation " x ==> g " := (in_language g x) (at level 60). (* ? *)
 
@@ -62,7 +62,7 @@ Theorem prefix_closed:
 Proof.
   unfold in_language, not.
   intros Q E g w w' H0 H1.
-  rewrite dist_extended_delta in H0. rewrite H1 in H0. apply H0.
+  rewrite dist_extended_transition in H0. rewrite H1 in H0. apply H0.
   destruct w'. reflexivity. reflexivity.
 Qed.
 
@@ -70,34 +70,32 @@ Qed.
 Example:
 
 Inductive states1 : Type :=
-  | q0 (* initial state *)
-  | q1
-  | q2 (* final state *).
+  q0 (* initial state *) |
+  q1 |
+  q2 (* final state *).
 
-Inductive events1 : Type :=
-  | a
-  | b.
+Inductive events1 : Type := a | b.
 
-Definition delta1 (q:states1) (e:events1) : state :=
+Definition transition1 (q:states1) (e:events1) : state :=
   match q, e with
-  | q0, a => proper_state q1
-  | q1, b => proper_state q2
-  | q2, a => proper_state q1
-  | _, _ => sink_state
+  q0, a => proper_state q1 |
+  q1, b => proper_state q2 |
+  q2, a => proper_state q1 |
+  _, _ => sink_state
   end.
 
-Definition is_final1 (q:states1) : bool :=
+Definition is_marked1 (q:states1) : bool :=
   match q with
-  | q2 => true
-  | _ => false
+  q2 => true |
+  _ => false
   end.
 
 Definition dfa1 :=
-  {| delta := delta1; initial_state := q0; is_final := is_final1 |}.
+  {| transition := transition1; initial_state := q0; is_marked := is_marked1 |}.
 
 Check dfa1.
 
-Compute extended_delta dfa1 (proper_state q0) [a;b;a;b;a;b].
+Compute extended_transition dfa1 (proper_state q0) [a;b;a;b;a;b].
 
 Theorem dfa1_test1 : [a;b;a;b;a;b] ==> dfa1.
 Proof.
